Proven validity of insert_element

bloom-filter/BloomFilter.fst
@@ -142,5 +142,5 @@ let insert_element bf e =
 val remove_element: bf:bloom_storage_u8 -> element -> Tot bloom_storage_u8
 let remove_element bf e =
   let hash_e = hash e in
-  let new_bf = { bf with ghost_state = spec_remove_element bf.ghost_state e } in
+  (* *) let new_bf = { bf with ghost_state = spec_remove_element bf.ghost_state e } in
   remove_hash new_bf hash_e
