bloom-filter/Proof.BloomFilter.fst
@@ -12,78 +12,92 @@ open Rust
 open Spec.BloomFilter
 open BloomFilter
 
-let modified_only_one_slot
-  (old_bf:bloom_storage_u8)
-  (new_bf:bloom_storage_u8)
-  (idx:valid_index) =
-  forall (idx':valid_index{idx <> idx'}).
-  slot_value new_bf idx' = slot_value old_bf idx'
+(**** Adjust slot properties ****)
 
-let adjust_slot_lemma
-  (bf:bloom_storage_u8)
-  (idx:valid_index)
-  (increment:bool{valid_incr bf idx increment})
-  : Lemma (ensures (
+let modified_only_one_slot (old_bf:bloom_storage_u8) (new_bf:bloom_storage_u8) (idx:valid_index) =
+  forall (idx':valid_index{idx <> idx'}). slot_value new_bf idx' = slot_value old_bf idx'
+
+let adjust_slot_lemma (bf:bloom_storage_u8) (idx:valid_index)
+  (increment:bool{valid_incr bf idx increment}) : Lemma (ensures (
     let new_bf = adjust_slot bf idx increment in
     modified_only_one_slot bf new_bf idx /\
-    begin if increment then
-      not (slot_is_empty new_bf idx)
-    else
-      true
-    end
+    begin if increment then not (slot_is_empty new_bf idx) else true end
   )) = ()
 
-let adjust_first_slot_lemma
-  (bf:bloom_storage_u8)
-  (hash:u32)
-  (increment:bool{valid_incr bf (first_slot_index hash) increment})
-  : Lemma (ensures (
+let adjust_first_slot_lemma (bf:bloom_storage_u8) (hash:u32)
+  (increment:bool{valid_incr bf (first_slot_index hash) increment}) : Lemma (ensures (
     let new_bf = adjust_first_slot bf hash increment in
     let idx = first_slot_index hash in
     modified_only_one_slot bf new_bf idx /\
-    begin if increment then
-      not (slot_is_empty new_bf idx)
-    else
-      true
-    end
+    begin if increment then not (slot_is_empty new_bf idx) else true end
   )) = adjust_slot_lemma bf (first_slot_index hash) increment
 
-let adjust_second_slot_lemma
-  (bf:bloom_storage_u8)
-  (hash:u32)
-  (increment:bool{valid_incr bf (second_slot_index hash) increment})
-  : Lemma (ensures (
+let adjust_second_slot_lemma (bf:bloom_storage_u8) (hash:u32)
+  (increment:bool{valid_incr bf (second_slot_index hash) increment}) : Lemma (ensures (
     let new_bf = adjust_second_slot bf hash increment in
     let idx = second_slot_index hash in
     modified_only_one_slot bf new_bf idx /\
-    begin if increment then
-      not (slot_is_empty new_bf idx)
-    else
-      true
-    end
+    begin if increment then not (slot_is_empty new_bf idx) else true end
   )) = adjust_slot_lemma bf (second_slot_index hash) increment
 
 
-let modified_hash_slots
-  (old_bf:bloom_storage_u8)
-  (new_bf:bloom_storage_u8)
-  (hash:u32) =
+(**** Insert hash properties ****)
+
+let modified_hash_slots (old_bf:bloom_storage_u8) (new_bf:bloom_storage_u8) (hash:u32) =
   let idx1 = first_slot_index hash in
   let idx2 = second_slot_index hash in
   forall (idx':valid_index{idx' <> idx1 /\ idx' <> idx2}).
   slot_value new_bf idx' = slot_value old_bf idx'
 
-let insert_hash_lemma
-  (bf:bloom_storage_u8)
-  (hash:u32)
-  : Lemma (ensures (
+let insert_hash_prelim_lemma (bf: bloom_storage_u8) (idx: valid_index)
+  : Lemma (requires (U8.v (slot_value bf idx) < _MAX_U8))
+    (ensures (U8.v (slot_value (adjust_slot bf idx true) idx) = U8.v (slot_value bf idx) + 1))
+  = ()
+
+let increase_or_saturate (old_bf:bloom_storage_u8) (new_bf:bloom_storage_u8) (idx:valid_index) =
+  if U8.v (slot_value old_bf idx) = _MAX_U8 then
+    U8.v (slot_value new_bf idx) = _MAX_U8
+  else
+    U8.(slot_value new_bf idx >^ slot_value old_bf idx)
+
+let insert_hash_lemma1 (bf: bloom_storage_u8) (hash:u32)
+  : Lemma (ensures (increase_or_saturate bf (insert_hash bf hash) (first_slot_index hash)))
+  = let idx1 = first_slot_index hash in let idx2 = second_slot_index hash in
+  let bf0 = adjust_first_slot bf hash true in
+  adjust_first_slot_lemma bf hash true; adjust_second_slot_lemma bf0 hash true;
+  if U8.v (slot_value bf idx1) = _MAX_U8 then () else begin
+    insert_hash_prelim_lemma bf idx1;
+    if idx1 = idx2 then if U8.v (slot_value bf0 idx1) = _MAX_U8 then () else
+        insert_hash_prelim_lemma bf0 idx1
+    else ()
+  end
+
+let insert_hash_lemma2 (bf: bloom_storage_u8) (hash:u32)
+  : Lemma (ensures (increase_or_saturate bf (insert_hash bf hash) (second_slot_index hash)))
+  = let idx1 = first_slot_index hash in let idx2 = second_slot_index hash in
+  let bf0 = adjust_first_slot bf hash true in
+  adjust_first_slot_lemma bf hash true; adjust_second_slot_lemma bf0 hash true;
+  if U8.v (slot_value bf idx2) = _MAX_U8 then () else begin
+    insert_hash_prelim_lemma bf idx2;
+    if U8.v (slot_value bf0 idx2) = _MAX_U8 then () else
+        insert_hash_prelim_lemma bf0 idx2
+  end
+
+let insert_hash_lemma (bf:bloom_storage_u8) (hash:u32) : Lemma (ensures (
     let new_bf = insert_hash bf hash in
+    let idx1 = first_slot_index hash in
+    let idx2 = second_slot_index hash in
     modified_hash_slots bf new_bf hash /\
-    might_contain_hash new_bf hash
-  )) =
-    adjust_first_slot_lemma bf hash true;
-    let bf0 = adjust_first_slot bf hash true in
-    adjust_second_slot_lemma bf0 hash true
+    might_contain_hash new_bf hash /\
+    increase_or_saturate bf new_bf idx1 /\
+    increase_or_saturate bf new_bf idx2
+  )) = adjust_first_slot_lemma bf hash true;
+  let bf0 = adjust_first_slot bf hash true in
+  adjust_second_slot_lemma bf0 hash true;
+  insert_hash_lemma1 bf hash;
+  insert_hash_lemma2 bf hash
+
+(**** Remove hash properties ****)
 
 let remove_hash_lemma
   (bf:bloom_storage_u8)
@@ -100,14 +114,7 @@ let remove_hash_lemma
     else
       adjust_second_slot_lemma bf0 hash false
 
-let add_only_bloom_filter
-  (bf:bloom_storage_u8)
-  : Tot bool =
-  let elements = bf.ghost_state.elements in
-  all_elements elements (fun e ->
-    might_contain_hash bf (hash e)
-  )
-
+(**** Insert element properties ****)
 
 let element_invalidation (bf: bloom_storage_u8) =
   (forall (e:element). (
@@ -119,153 +126,28 @@ let count_invariant_property (bf:bloom_storage_u8) (e:element) : Tot bool =
   let hash_e = hash e in
   let val1 = slot_value bf (first_slot_index hash_e) in
   let val2 = slot_value bf (second_slot_index hash_e) in
-  begin if U8.v val1 < _MAX_U8 then true else
+  begin if U8.v val1 = _MAX_U8 then true else
     element_count bf.ghost_state.elements e <= U8.v val1
-  end && begin if U8.v val2 < _MAX_U8 then true else
+  end && begin if U8.v val2 = _MAX_U8 then true else
     element_count bf.ghost_state.elements e <= U8.v val2
   end
 
-let count_invariant (bf:bloom_storage_u8) : Tot bool =
-  all_elements #element bf.ghost_state.elements (fun e ->
-    count_invariant_property bf e
-  )
-
-let lemma_add_only_bloom_filter
-  (bf: bloom_storage_u8)
-  : Lemma (ensures (
-    add_only_bloom_filter bf <==>
-    (forall (e:element{contains bf.ghost_state.elements e}).
-      might_contain_hash bf (hash e))
-  )) =
-    all_elements_lemma
-      #element
-      bf.ghost_state.elements
-      (fun e -> might_contain_hash bf (hash e))
-
-let lemma_count_invariant (bf:bloom_storage_u8)
-  : Lemma (ensures (count_invariant bf <==>
-    (forall (e:element{contains bf.ghost_state.elements e}).
+let count_invariant (bf:bloom_storage_u8) =
+   (forall (e:element{contains bf.ghost_state.elements e}).
     count_invariant_property bf e)
-  )) =
-  all_elements_lemma #element bf.ghost_state.elements
-   (fun e -> count_invariant_property bf e)
 
-type valid_bloom_storage_u8 = bf:bloom_storage_u8{element_invalidation bf /\ count_invariant bf}
+let valid_bf (bf:bloom_storage_u8) = element_invalidation bf /\ count_invariant bf
 
-type add_only_bloom_storage_u8 = bf:valid_bloom_storage_u8{add_only_bloom_filter bf}
-
-let lemma_insert_hash_prelim1 (bf: bloom_storage_u8) (idx: valid_index)
-  : Lemma (requires (U8.v (slot_value bf idx) < _MAX_U8))
-    (ensures (U8.v (slot_value (adjust_slot bf idx true) idx) = U8.v (slot_value bf idx) + 1))
-  = ()
-
-let lemma_insert_hash_prelim2 (bf: bloom_storage_u8) (idx: valid_index)
-  : Lemma (requires (U8.v (slot_value bf idx) = _MAX_U8))
-    (ensures (U8.v (slot_value (adjust_slot bf idx true) idx) = _MAX_U8))
-  = ()
-
-let lemma_insert_hash_non_saturating1 (bf: bloom_storage_u8) (hash:u32)
-  : Lemma (requires (
-      U8.v (slot_value bf (first_slot_index hash)) < _MAX_U8)
-    )
-    (ensures (
-      U8.v (slot_value (insert_hash bf hash) (first_slot_index hash)) >
-	U8.v (slot_value bf (first_slot_index hash))
-    )) =
-    let idx1 = first_slot_index hash in let idx2 = second_slot_index hash in
-    lemma_insert_hash_prelim1 bf idx1;
-    let bf0 = adjust_first_slot bf hash true in
-    adjust_first_slot_lemma bf hash true; adjust_second_slot_lemma bf0 hash true;
-    if idx1 = idx2 then begin
-      if U8.v (slot_value bf0 idx1) = _MAX_U8 then
-        lemma_insert_hash_prelim2 bf0 idx1
-      else
-        lemma_insert_hash_prelim1 bf0 idx1
-    end else ()
-
-let lemma_insert_hash_non_saturating2 (bf: bloom_storage_u8) (hash:u32)
-  : Lemma (requires (
-      U8.v (slot_value bf (second_slot_index hash)) < _MAX_U8)
-    )
-    (ensures (
-      U8.v (slot_value (insert_hash bf hash) (second_slot_index hash)) >
-	U8.v (slot_value bf (second_slot_index hash))
-    )) =
-    let idx1 = first_slot_index hash in let idx2 = second_slot_index hash in
-    lemma_insert_hash_prelim1 bf idx2;
-    let bf0 = adjust_first_slot bf hash true in
-    adjust_first_slot_lemma bf hash true; adjust_second_slot_lemma bf0 hash true;
-    if idx1 = idx2 then begin
-      if U8.v (slot_value bf0 idx2) = _MAX_U8 then
-        lemma_insert_hash_prelim2 bf0 idx1
-      else
-        lemma_insert_hash_prelim1 bf0 idx1
-    end else ()
-
-(*
- (* *) lemma_count_invariant bf;
-  (* *) lemma_count_invariant new_bf;
-  let inner_lemma
-    (e':element{contains new_bf.ghost_state.elements e'})
-    : Lemma (ensures (count_invariant_property new_bf e'))
-  =
-    let hash_e' = hash e' in
-    let idx1_e = first_slot_index (hash e) in
-    let idx1_e' = first_slot_index (hash e') in
-    let idx2_e = second_slot_index (hash e) in
-    let idx2_e' = second_slot_index (hash e') in
-    let new_val1 = slot_value new_bf idx1_e' in
-    let new_val2 = slot_value new_bf idx2_e'  in
-    let old_val1 = slot_value bf idx1_e' in
-    let old_val2 = slot_value bf idx2_e' in
-    if U8.v old_val1 = _MAX_U8 then () else
-    assert(U8.v old_val1 < _MAX_U8);
-    begin if idx1_e' = idx1_e || idx1_e' = idx2_e then begin
-      Classical.or_elim
-        #(idx1_e' = idx1_e)
-        #(idx1_e' = idx2_e)
-        #(fun _ -> U8.(old_val1 <=^ new_val1))
-        (fun _ ->
-	  //admit();
-	  lemma_insert_hash_prelim bf idx1_e;
-	  admit()
-	)
-        (fun _ ->
-	  admit();
-	  lemma_insert_hash_prelim bf idx2_e;
-	  admit()
-	);
-       admit()
-    end else
-      admit()
-    end;
-    admit()
+let insert_element_lemma (bf:bloom_storage_u8) (e:element)
+  : Lemma (requires (valid_bf bf)) (ensures (valid_bf (insert_element bf e)))
+  = let new_bf = insert_element bf e in let hash_e = hash e in
+  insert_hash_lemma bf hash_e;
+  let forall_intro_lemma (e':element{contains new_bf.ghost_state.elements e'})
+    : Lemma (ensures (count_invariant_property new_bf e')) =
+    assert(count_invariant_property bf e')
+  in Classical.forall_intro forall_intro_lemma
 
 
-(*
-    begin if U8.v val1 < _MAX_U8 then () else
-     begin if idx1_e' = idx1_e || idx1_e' = idx2_e then begin
-       if U8.v (slot_value bf idx1_e') < _MAX_U8 then
-         admit()
-       else
-         assert(U8.v (slot_value new_bf idx1_e') = _MAX_U8);
-	 assert(U8.v val1 = _MAX_U8 /\ U8.v val1 < _MAX_U8);
-	 lemma_contradiction new_bf e' val1;
-	 admit()
-       end else begin
-         assert(slot_value bf idx1_e' = slot_value new_bf idx1_e');
-	 assert(count_invariant_property bf e');
-	 assert(element_count bf.ghost_state.elements e' <= U8.v val1)
-       end
-     end
-     //assume(element_count new_bf.ghost_state.elements e' <= U8.v val1)
-    end;
-    begin if U8.v val2 < _MAX_U8 then () else
-      assume(element_count new_bf.ghost_state.elements e' <= U8.v val2)
-    end
- *)
-  in
-  (* *) Classical.forall_intro inner_lemma;
-  (* *) lemma_add_only_bloom_filter bf;
-  (* *) lemma_add_only_bloom_filter new_bf;
-  *)
+let remove_element_lemma_element_invalidation (bf:bloom_storage_u8) (e:element)
+  : Lemma(requires (valid_bf bf)) (ensures (element_invalidation (remove_element bf e))) =
+ admit()
